SStructTT.lean
@@ -4,7 +4,8 @@ import SStructTT.Defs.ARS
 import SStructTT.Defs.Subst
 import SStructTT.Defs.SStruct
 import SStructTT.Defs.Syntax
-import SStructTT.Defs.Context
 
+import SStructTT.Static.Context
 import SStructTT.Static.Step
 import SStructTT.Static.Confluence
+import SStructTT.Static.Typed
