SStructTT/Static/Context.lean
@@ -1,0 +1,10 @@
+import SStructTT.Defs.Syntax
+
+abbrev Ctx Srt := List (Tm Srt)
+
+inductive Has {Srt} : Ctx Srt -> Var -> Tm Srt -> Prop where
+  | zero Γ A :
+    Has (A :: Γ) 0 A.[shift 1]
+  | succ Γ A B x :
+    Has Γ x A ->
+    Has (B :: Γ) x.succ A.[shift 1]
