SStructTT/Static/Typed.lean
@@ -1,0 +1,102 @@
+import SStructTT.Defs.SStruct
+import SStructTT.Defs.Syntax
+import SStructTT.Static.Confluence
+import SStructTT.Static.Context
+
+namespace Static
+variable {Srt : Type} [SStruct Srt]
+
+mutual
+inductive Typed : Ctx Srt -> Tm Srt -> Tm Srt -> Prop where
+  | srt Γ i :
+    Wf Γ ->
+    Typed Γ (.srt s0 i) (.srt s0 (i.succ))
+  | var Γ x A :
+    Wf Γ ->
+    Has Γ x A ->
+    Typed Γ (.var x) A
+  | pi Γ A B r s sA sB iA iB :
+    Typed Γ A (.srt sA iA) ->
+    Typed (A :: Γ) B (.srt sB iB) ->
+    Typed Γ (.pi A B r s) (.srt s (max iA iB))
+  | lam Γ A B m r s sA iA :
+    Typed Γ A (.srt sA iA) ->
+    Typed (A :: Γ) m B ->
+    Typed Γ (.lam A m r s) (.pi A B r s)
+  | app Γ A B m n r s :
+    Typed Γ m (.pi A B r s) ->
+    Typed Γ n A ->
+    Typed Γ (.app m n) B.[n/]
+  | sig Γ A B r s sA sB iA iB :
+    Typed Γ A (.srt sA iA) ->
+    Typed (A :: Γ) B (.srt sB iB) ->
+    Typed Γ (.sig A B r s) (.srt s (max iA iB))
+  | pair Γ A B m n r s i :
+    Typed Γ (.pi A B r s) (.srt s i) ->
+    Typed Γ m A ->
+    Typed Γ n B.[m/] ->
+    Typed Γ (.pair m n r s) (.sig A B r s)
+  | proj Γ A B C m n r s sC iC :
+    Typed (.sig A B r s :: Γ) C (.srt sC iC) ->
+    Typed Γ m (.sig A B r s) ->
+    Typed (B :: A :: Γ) n C.[.pair (.var 1) (.var 0) r s .: shift 2] ->
+    Typed Γ (.proj C m n) C.[m/]
+  | bool Γ :
+    Wf Γ ->
+    Typed Γ .bool (.srt s0 0)
+  | tt Γ :
+    Wf Γ ->
+    Typed Γ .tt .bool
+  | ff Γ :
+    Wf Γ ->
+    Typed Γ .ff .bool
+  | ite Γ A m n1 n2 s i :
+    Typed (.bool :: Γ) A (.srt s i) ->
+    Typed Γ m .bool ->
+    Typed Γ n1 A.[.tt/] ->
+    Typed Γ n2 A.[.ff/] ->
+    Typed Γ (.ite A m n1 n2) A.[m/]
+  | id Γ A m n s i :
+    Typed Γ A (.srt s i) ->
+    Typed Γ m A ->
+    Typed Γ n A ->
+    Typed Γ  (.id A m n) (.srt s0 i)
+  | rfl Γ A m :
+    Typed Γ m A ->
+    Typed Γ (.rfl m) (.id A m m)
+  | rw Γ A B m n a b s i :
+    Typed (.id A.[shift 1] a.[shift 1] (.var 0) :: A :: Γ) B (.srt s i) ->
+    Typed Γ m B.[.rfl a,a/] ->
+    Typed Γ n (.id A a b) ->
+    Typed Γ (.rw B m n) B.[n,b/]
+  | conv Γ A B m s i :
+    A === B ->
+    Typed Γ m A ->
+    Typed Γ B (.srt s i) ->
+    Typed Γ m B
+
+inductive Wf : Ctx Srt -> Prop where
+  | nil : Wf []
+  | cons Γ A s i :
+    Typed Γ A (.srt s i) ->
+    Wf Γ ->
+    Wf (A :: Γ)
+end
+
+notation:50 Γ:50 " ⊢ " m:51 " : " A:51 => Typed Γ m A
+notation:50 Γ:50 " ⊢ " => Wf Γ
+
+-- Register non-mutual recursor as default.
+@[induction_eliminator]
+def Typed.rec_non_mutual {motive : ∀ Γ m a, @Typed Srt _ Γ m a -> Prop} :=
+  Typed.rec (motive_1 := motive) (motive_2 := fun _ _ => True)
+
+-- Register non-mutual recursor as default.
+@[induction_eliminator]
+def Wf.rec_non_mutual {motive : ∀ Γ, @Wf Srt _ Γ -> Prop} :=
+  Wf.rec (motive_1 := fun _ _ _ _ => True) (motive_2 := motive)
+
+lemma Typed.toWf (Γ : Ctx Srt) m A : Γ ⊢ m : A -> Γ ⊢ := by
+  intro h
+  induction h
+  all_goals trivial
